src/lowparse/LowParse.Low.BCVLI.fst
@@ -168,11 +168,126 @@ let serialize32_bcvli'
     len
   end
 
-#pop-options
-
 inline_for_extraction
 let serialize32_bcvli : serializer32 serialize_bcvli =
   fun (x: U32.t) #rrel #rel b pos -> serialize32_bcvli' x b pos
 
 let write_bcvli : leaf_writer_strong serialize_bcvli =
   leaf_writer_strong_of_serializer32 serialize32_bcvli ()
+
+let validate_bounded_bcvli'
+  (min32: U32.t)
+  (max32: U32.t { U32.v min32 <= U32.v max32 })
+: Tot (validator (parse_bounded_bcvli (U32.v min32) (U32.v max32)))
+= fun #rrel #rel input pos ->
+  let h = HST.get () in
+  [@inline_let] let _ =
+    valid_facts (parse_bounded_bcvli (U32.v min32) (U32.v max32)) h input pos;
+    parse_bounded_bcvli_eq (U32.v min32) (U32.v max32) (bytes_of_slice_from h input pos);
+    parse_bcvli_eq (bytes_of_slice_from h input pos);
+    valid_facts (parse_bounded_integer_le 1) h input pos
+  in
+  let pos1 = validate_total_constant_size (parse_bounded_integer_le 1) 1ul () input pos in
+  if validator_max_length `U32.lt` pos1
+  then pos1
+  else
+    [@inline_let] let _ =
+      valid_facts (parse_bounded_integer_le 2) h input pos1;
+      valid_facts (parse_bounded_integer_le 4) h input pos1
+    in
+    let r = read_bounded_integer_le_1 input pos in
+    if r `U32.lt` 253ul && min32 `U32.lte` r && r `U32.lte` max32
+    then pos1
+    else if max32 `U32.lt` 253ul
+    then validator_error_generic
+    else if r = 253ul
+    then
+      if 65536ul `U32.lte` min32
+      then validator_error_generic
+      else
+        let pos2 = validate_total_constant_size (parse_bounded_integer_le 2) 2ul () input pos1 in
+        if validator_max_length `U32.lt` pos2
+        then pos2
+        else
+          (* because of the non-malleability constraint, I need to actually read the value and check whether it is not a lower integer *)
+          let r = read_bounded_integer_le_2 input pos1 in
+          if r `U32.lt` 253ul || r `U32.lt` min32 || max32 `U32.lt` r
+          then validator_error_generic
+          else pos2
+    else if max32 `U32.lt` 65536ul
+    then validator_error_generic
+    else if r = 254ul
+    then
+      let pos2 = validate_total_constant_size (parse_bounded_integer_le 4) 4ul () input pos1 in
+      if validator_max_length `U32.lt` pos2
+      then pos2
+      else
+        (* because of the non-malleability constraint, I need to actually read the value and check whether it is not a lower integer *)
+        let r = read_bounded_integer_le_4 input pos1 in
+        if r `U32.lt` 65536ul || r `U32.lt` min32 || max32 `U32.lt` r
+        then validator_error_generic
+        else pos2
+    else validator_error_generic
+
+inline_for_extraction
+noextract
+let validate_bounded_bcvli
+  (min: nat)
+  (min32: U32.t { U32.v min32 == min })
+  (max: nat { min <= max })
+  (max32: U32.t { U32.v max32 == max })
+: Tot (validator (parse_bounded_bcvli min max))
+= validate_bounded_bcvli' min32 max32
+
+inline_for_extraction
+noextract
+let jump_bounded_bcvli
+  (min: nat)
+  (max: nat { min <= max })
+: Tot (jumper (parse_bounded_bcvli min max))
+= fun #rrel #rel input pos ->
+    let h = HST.get () in
+    [@inline_let]
+    let _ =
+      valid_facts (parse_bounded_bcvli min max) h input pos;
+      parse_bounded_bcvli_eq min max (bytes_of_slice_from h input pos);
+      valid_facts parse_bcvli h input pos
+    in
+    jump_bcvli input pos
+
+inline_for_extraction
+noextract
+let read_bounded_bcvli
+  (min: nat)
+  (max: nat { min <= max })
+: Tot (leaf_reader (parse_bounded_bcvli min max))
+= fun #rrel #rel input pos ->
+    let h = HST.get () in
+    [@inline_let]
+    let _ =
+      valid_facts (parse_bounded_bcvli min max) h input pos;
+      parse_bounded_bcvli_eq min max (bytes_of_slice_from h input pos);
+      valid_facts parse_bcvli h input pos
+    in
+    read_bcvli input pos <: bounded_int32 min max
+
+inline_for_extraction
+noextract
+let serialize32_bounded_bcvli
+  (min: nat)
+  (max: nat { min <= max })
+: Tot (serializer32 (serialize_bounded_bcvli min max))
+= fun (x: bounded_int32 min max) #rrel #rel b pos ->
+    [@inline_let]
+    let _ = serialize_bounded_bcvli_eq min max x in
+    serialize32_bcvli x b pos
+
+inline_for_extraction
+noextract
+let write_bounded_bcvli
+  (min: nat)
+  (max: nat { min <= max })
+: Tot (leaf_writer_strong (serialize_bounded_bcvli min max))
+= leaf_writer_strong_of_serializer32 (serialize32_bounded_bcvli min max) ()
+
+#pop-options
