src/lowparse/LowParse.SLow.BCVLI.fst
@@ -71,4 +71,79 @@ let size32_bcvli
     else 5ul
   ) <: (res: _ { size32_postcond serialize_bcvli x res } ))
 
+inline_for_extraction
+let parse32_bounded_bcvli
+  (min: nat)
+  (min32: U32.t { U32.v min32 == min })
+  (max: nat { min <= max })
+  (max32: U32.t { U32.v max32 == max })
+: Tot (parser32 (parse_bounded_bcvli min max))
+= fun input -> ((
+    [@inline_let]
+    let _ = parse_bounded_bcvli_eq min max (B32.reveal input) in
+    [@inline_let]
+    let _ = parse_bcvli_eq (B32.reveal input) in
+    match parse32_bounded_integer_le_1 input with
+    | None -> None
+    | Some (x32, consumed_x) ->
+      if x32 `U32.lt` 253ul && min32 `U32.lte` x32 && x32 `U32.lte` max32
+      then Some (x32, consumed_x)
+      else if max32 `U32.lt` 253ul
+      then None
+      else
+        if x32 = 253ul
+        then
+          if 65536ul `U32.lte` min32
+          then None
+          else
+            let input' = B32.slice input consumed_x (B32.len input) in
+            match parse32_bounded_integer_le_2 input' with
+            | None -> None
+            | Some (y, consumed_y) ->
+              if
+                y `U32.lt` 253ul || y `U32.lt` min32 || max32 `U32.lt` y
+              then
+                None
+              else
+                Some (y, consumed_x `U32.add` consumed_y)
+        else if max32 `U32.lt` 65536ul
+        then None
+        else if x32 = 254ul
+        then
+          let input' = B32.slice input consumed_x (B32.len input) in
+          match parse32_bounded_integer_le_4 input' with
+          | None -> None
+          | Some (y, consumed_y) ->
+            if
+              y `U32.lt` 65536ul || y `U32.lt` min32 || max32 `U32.lt` y
+            then
+              None
+            else
+              Some (y, consumed_x `U32.add` consumed_y)
+        else
+          None
+  ) <: (res: _ { parser32_correct (parse_bounded_bcvli min max) input res }))
+
+inline_for_extraction
+let serialize32_bounded_bcvli
+  (min: nat)
+  (max: nat { min <= max })
+: Tot (serializer32 (serialize_bounded_bcvli min max))
+= fun x -> ((
+    [@inline_let]
+    let _ = serialize_bounded_bcvli_eq min max x in
+    serialize32_bcvli x
+  ) <: (res: _ { serializer32_correct (serialize_bounded_bcvli min max) x res }))
+
+inline_for_extraction
+let size32_bounded_bcvli
+  (min: nat)
+  (max: nat { min <= max })
+: Tot (size32 (serialize_bounded_bcvli min max))
+= fun x -> ((
+    [@inline_let]
+    let _ = serialize_bounded_bcvli_eq min max x in
+    size32_bcvli x
+  ) <: (res: _ { size32_postcond (serialize_bounded_bcvli min max) x res }))
+
 #pop-options
